# distance from a point to a line

::: {show-in="html"}
點到直線距離
:::

::: {show-in="pdf"}
\begin{CJK}{UTF8}{bsmi}
點到直線距離
\end{CJK}
:::

::: {.theorem #unnamed-chunk-1}
$$
\begin{array}{c}
\begin{cases}
P=P\left(x_{0},y_{0}\right)\\
L=L\left(x,y\right)=Ax+By+C=0,A^{2}+B^{2}\ne0
\end{cases}\\
\Downarrow\\
d\left(P,L\right)=\dfrac{\left|Ax_{0}+By_{0}+C\right|}{\sqrt{A^{2}+B^{2}}}
\end{array}
$$
:::

https://en.wikipedia.org/wiki/Distance_from_a_point_to_a_line

https://highscope.ch.ntu.edu.tw/wordpress/?p=47407

https://web.math.sinica.edu.tw/mathmedia/HTMLarticle18.jsp?mID=40312

Proofs:

## by shortest $\overline{PP^{\prime}}$

$$
\begin{aligned}
 & P^{\prime}=P^{\prime}\left(x,y\right)\in L=Ax+By+C=0\\
\Rightarrow & y=\dfrac{-1}{B}\left(Ax+C\right)
\end{aligned}
$$


$$
\begin{aligned}
\overline{PP^{\prime}}^{2}\left(x,y\right)= & \left(x_{0}-x\right)^{2}+\left(y_{0}-y\right)^{2}\\
= & \left(x_{0}-x\right)^{2}+\left(y_{0}-\dfrac{-1}{B}\left(Ax+C\right)\right)^{2}\\
= & \left(x-x_{0}\right)^{2}+\left(\dfrac{A}{B}x+\dfrac{C}{B}+y_{0}\right)^{2}=\overline{PP^{\prime}}^{2}\left(x\right)
\end{aligned}
$$

$$
\begin{aligned}
0=\dfrac{\partial}{\partial x}\overline{PP^{\prime}}^{2}\left(x\right)= & 2\left(x-x_{0}\right)+2\left(\dfrac{A}{B}x+\dfrac{C}{B}+y_{0}\right)\dfrac{A}{B}\\
= & \dfrac{2}{B^{2}}\left(B^{2}\left(x-x_{0}\right)+A^{2}x+AC+ABy_{0}\right)\\
= & \dfrac{2}{B^{2}}\left[\left(A^{2}+B^{2}\right)x-\left(B^{2}x_{0}-ABy_{0}-AC\right)\right]\\
x= & \dfrac{B^{2}x_{0}-ABy_{0}-AC}{A^{2}+B^{2}}
\end{aligned}
$$
or by completing the square to find $x$.

$$
\begin{aligned}
 & \overline{PP^{\prime}}^{2}\left(x=\dfrac{B^{2}x_{0}-ABy_{0}-AC}{A^{2}+B^{2}}\right)\\
= & \left(\dfrac{B^{2}x_{0}-ABy_{0}-AC}{A^{2}+B^{2}}-x_{0}\right)^{2}+\left(\dfrac{A}{B}\dfrac{B^{2}x_{0}-ABy_{0}-AC}{A^{2}+B^{2}}+\dfrac{C}{B}+y_{0}\right)^{2}\\
= & \left(\dfrac{-A^{2}x_{0}-ABy_{0}-AC}{A^{2}+B^{2}}\right)^{2}+\left(\dfrac{A\left(B^{2}x_{0}-ABy_{0}-AC\right)+C\left(A^{2}+B^{2}\right)+B\left(A^{2}+B^{2}\right)y_{0}}{B\left(A^{2}+B^{2}\right)}\right)^{2}\\
= & \left(\dfrac{-A\left(Ax_{0}+By_{0}+C\right)}{A^{2}+B^{2}}\right)^{2}+\left(\dfrac{AB^{2}x_{0}+B^{3}y_{0}+B^{2}C}{B\left(A^{2}+B^{2}\right)}\right)^{2}\\
= & \dfrac{A^{2}\left(Ax_{0}+By_{0}+C\right)^{2}}{\left(A^{2}+B^{2}\right)^{2}}+\dfrac{B^{2}\left(Ax_{0}+By_{0}+C\right)^{2}}{\left(A^{2}+B^{2}\right)^{2}}\\
= & \dfrac{\left(Ax_{0}+By_{0}+C\right)^{2}}{A^{2}+B^{2}}\\
\overline{PP^{\prime}}= & \overline{PP^{\prime}}\left(x=\dfrac{B^{2}x_{0}-ABy_{0}-AC}{A^{2}+B^{2}}\right)=\dfrac{\left|Ax_{0}+By_{0}+C\right|}{\sqrt{A^{2}+B^{2}}}
\end{aligned}
$$

## by perpendicular foot

$$
y=\dfrac{-A}{B}x-\dfrac{C}{B}=\dfrac{-1}{B}\left(Ax+C\right),\text{ if }B\ne0
$$

$$
L_{\perp}:\left(y=\dfrac{B}{A}x+K\right)\perp\left(y=\dfrac{-A}{B}x-\dfrac{C}{B}\right):L
$$

$$
L_{\perp}=L_{\perp}\left(x,y\right)=Bx-Ay+K=0
$$
$$
P=P\left(x_{0},y_{0}\right)\in L_{\perp}=B\left(x-x_{0}\right)-A\left(y-y_{0}\right)=0
$$

$$
L_{\perp}=Bx-Ay-\left(Bx_{0}-Ay_{0}\right)=0
$$
perpendicular foot = foot of the perpendicular $P^{\prime}$

$$
\begin{aligned}
P^{\prime}\in\left(L_{\perp}\cap L\right)= & \begin{cases}
L=Ax+By+C=0\\
L_{\perp}=Bx-Ay-\left(Bx_{0}-Ay_{0}\right)=0
\end{cases}\\
= & \begin{cases}
Ax+By=-C\\
Bx-Ay=Bx_{0}-Ay_{0}
\end{cases}\\
P^{\prime}=P^{\prime}\left(x,y\right)= & \left(\dfrac{\begin{vmatrix}-C & B\\
Bx_{0}-Ay_{0} & -A
\end{vmatrix}}{\begin{vmatrix}A & B\\
B & -A
\end{vmatrix}},\dfrac{\begin{vmatrix}A & -C\\
B & Bx_{0}-Ay_{0}
\end{vmatrix}}{\begin{vmatrix}A & B\\
B & -A
\end{vmatrix}}\right)\\
= & \left(\dfrac{\begin{vmatrix}C & B\\
-Bx_{0}+Ay_{0} & -A
\end{vmatrix}}{\begin{vmatrix}A & -B\\
B & A
\end{vmatrix}},\dfrac{\begin{vmatrix}A & C\\
B & -Bx_{0}+Ay_{0}
\end{vmatrix}}{\begin{vmatrix}A & -B\\
B & A
\end{vmatrix}}\right)\\
= & \left(\dfrac{B^{2}x_{0}-ABy_{0}-AC}{A^{2}+B^{2}},\dfrac{-ABx_{0}+A^{2}y_{0}-BC}{A^{2}+B^{2}}\right)
\end{aligned}
$$

$$
\begin{aligned}
 & d\left(P,L\right)=\overline{PP^{\prime}}\\
= & \left\Vert \left(x_{0},y_{0}\right)-\left(\dfrac{B^{2}x_{0}-ABy_{0}-AC}{A^{2}+B^{2}},\dfrac{-ABx_{0}+A^{2}y_{0}-BC}{A^{2}+B^{2}}\right)\right\Vert \\
= & \sqrt{\left(x_{0}-\dfrac{B^{2}x_{0}-ABy_{0}-AC}{A^{2}+B^{2}}\right)^{2}+\left(y_{0}-\dfrac{-ABx_{0}+A^{2}y_{0}-BC}{A^{2}+B^{2}}\right)^{2}}\\
= & \sqrt{\left(\dfrac{A^{2}x_{0}+ABy_{0}+AC}{A^{2}+B^{2}}\right)^{2}+\left(\dfrac{ABx_{0}+B^{2}y_{0}+BC}{A^{2}+B^{2}}\right)^{2}}\\
= & \sqrt{\dfrac{A^{2}\left(Ax_{0}+By_{0}+C\right)^{2}+B^{2}\left(Ax_{0}+By_{0}+C\right)^{2}}{\left(A^{2}+B^{2}\right)^{2}}}=\sqrt{\dfrac{\left(Ax_{0}+By_{0}+C\right)^{2}}{A^{2}+B^{2}}}\\
= & \dfrac{\left|Ax_{0}+By_{0}+C\right|}{\sqrt{A^{2}+B^{2}}}
\end{aligned}
$$

## by normal vector

$$
\begin{cases}
\overset{\rightharpoonup}{n}=\left(A,B\right)\perp L=Ax+By+C=0\\
\overset{\rightharpoonup}{PP^{\prime}}=P^{\prime}-P=\left(x-x_{0},y-y_{0}\right)
\end{cases}
$$

::: {show-in="html"}

$P$到$L$的距離$d\left(P,L\right)$即為$L$線上一點$P^{\prime}$對應之$\overset{\rightharpoonup}{PP^{\prime}}$在$L$法向量$\overset{\rightharpoonup}{n}$方向上的投影長

:::

::: {show-in="pdf"}

\begin{CJK}{UTF8}{bsmi}
$P$到$L$的距離$d\left(P,L\right)$即為$L$線上一點$P^{\prime}$對應之$\overset{\rightharpoonup}{PP^{\prime}}$在$L$法向量$\overset{\rightharpoonup}{n}$方向上的投影長
\end{CJK}

:::

$$
\begin{aligned}
\overset{\rightharpoonup}{PP^{\prime}}\cdot\overset{\rightharpoonup}{n}= & \left\Vert \overset{\rightharpoonup}{PP^{\prime}}\right\Vert \left\Vert \overset{\rightharpoonup}{n}\right\Vert \cos\theta\\
\left|\overset{\rightharpoonup}{PP^{\prime}}\cdot\overset{\rightharpoonup}{n}\right|= & \left\Vert \overset{\rightharpoonup}{PP^{\prime}}\right\Vert \left\Vert \overset{\rightharpoonup}{n}\right\Vert \left|\cos\theta\right|\\
\left\Vert \overset{\rightharpoonup}{PP^{\prime}}\right\Vert \left|\cos\theta\right|= & \left|\overset{\rightharpoonup}{PP^{\prime}}\cdot\widehat{\boldsymbol{n}}\right|=\dfrac{\left|\overset{\rightharpoonup}{PP^{\prime}}\cdot\overset{\rightharpoonup}{n}\right|}{\left\Vert \overset{\rightharpoonup}{n}\right\Vert }=\dfrac{\left|\left(x-x_{0},y-y_{0}\right)\cdot\left(A,B\right)\right|}{\left\Vert \left(A,B\right)\right\Vert }\\
= & \dfrac{\left|A\left(x-x_{0}\right)+B\left(y-y_{0}\right)\right|}{\sqrt{A^{2}+B^{2}}}=\dfrac{\left|-Ax_{0}-By_{0}+Ax+By\right|}{\sqrt{A^{2}+B^{2}}}\\
\begin{subarray}{c}
Ax+By+C=0\\
=\\
Ax+By=-C
\end{subarray} & \dfrac{\left|-Ax_{0}-By_{0}-C\right|}{\sqrt{A^{2}+B^{2}}}=\dfrac{\left|Ax_{0}+By_{0}+C\right|}{\sqrt{A^{2}+B^{2}}}
\end{aligned}
$$

PDF LaTeX `\usepackage{fdsymbol}` to have `\overrightharpoon` vector; however, there are too many side effects, including ugly mathptmx $\sum$, ...

```
\usepackage{fdsymbol} % vector over accent, but will use mathptmx
% replace the rather ugly mathptmx \sum operator with the equivalent Computer Modern one
\let\sum\relax
\DeclareSymbolFont{CMlargesymbols}{OMX}{cmex}{m}{n}
\DeclareMathSymbol{\sum}{\mathop}{CMlargesymbols}{"50}
```

## by Cauchy inequality

$$
\begin{aligned}
Ax+By+C= & 0\\
Ax+By= & -C\\
\left(Ax+By\right)-\left(Ax_{0}+By_{0}\right)= & -C-\left(Ax_{0}+By_{0}\right)\\
A\left(x-x_{0}\right)+B\left(y-y_{0}\right)= & -\left(Ax_{0}+By_{0}+C\right)
\end{aligned}
$$

$$
\begin{aligned}
\overline{PP^{\prime}}^{2}= & \left(x_{0}-x\right)^{2}+\left(y_{0}-y\right)^{2}\\
\left[A^{2}+B^{2}\right]\overline{PP^{\prime}}^{2}= & \left[A^{2}+B^{2}\right]\left[\left(x_{0}-x\right)^{2}+\left(y_{0}-y\right)^{2}\right]\\
\ge & \left[A\left(x-x_{0}\right)+B\left(y-y_{0}\right)\right]^{2}\\
= & \left[-\left(Ax_{0}+By_{0}+C\right)\right]^{2}=\left(Ax_{0}+By_{0}+C\right)^{2}\\
\overline{PP^{\prime}}^{2}\ge & \dfrac{\left(Ax_{0}+By_{0}+C\right)^{2}}{A^{2}+B^{2}}\\
\overline{PP^{\prime}}\ge & \dfrac{\left|Ax_{0}+By_{0}+C\right|}{\sqrt{A^{2}+B^{2}}}
\end{aligned}
$$
