# determinant

::: {show-in="html"}
<iframe width=500 height=300 frameborder="0" allowfullscreen src="https://player.bilibili.com/player.html?bvid=BV13e411m7Js&autoplay=0"></iframe>
:::

::: {show-in="html"}
<iframe width=500 height=300 frameborder="0" allowfullscreen src="https://www.youtube.com/embed/Sv7VseMsOQc"></iframe>
:::

## induction of determinant axioms

## determinant axioms

determinant axioms

$$
\begin{aligned}
 & \begin{cases}
\begin{cases}
\det\left(\boldsymbol{u},\boldsymbol{v}\right)=\det\left(\boldsymbol{u}+s\boldsymbol{v},\boldsymbol{v}\right)\\
\det\left(\boldsymbol{u},\boldsymbol{v}\right)=\det\left(\boldsymbol{u},\boldsymbol{v}+s\boldsymbol{u}\right)
\end{cases} & \text{translation invariance}\\
\begin{cases}
\det\left(s\boldsymbol{u},\boldsymbol{v}\right)=s\det\left(\boldsymbol{u},\boldsymbol{v}\right)\\
\det\left(\boldsymbol{u},s\boldsymbol{v}\right)=s\det\left(\boldsymbol{u},\boldsymbol{v}\right)
\end{cases} & \text{scaling}\\
\begin{cases}
\det\left(\boldsymbol{u}_{{\scriptscriptstyle 1}}+\boldsymbol{u}_{{\scriptscriptstyle 2}},\boldsymbol{v}\right)=\det\left(\boldsymbol{u}_{{\scriptscriptstyle 1}},\boldsymbol{v}\right)+\det\left(\boldsymbol{u}_{{\scriptscriptstyle 2}},\boldsymbol{v}\right)\\
\det\left(\boldsymbol{u},\boldsymbol{v}_{{\scriptscriptstyle 1}}+\boldsymbol{v}_{{\scriptscriptstyle 2}}\right)=\det\left(\boldsymbol{u},\boldsymbol{v}_{{\scriptscriptstyle 1}}\right)+\det\left(\boldsymbol{u},\boldsymbol{v}_{{\scriptscriptstyle 2}}\right)
\end{cases} & \text{decomposition}
\end{cases}\\
\Leftrightarrow & \begin{cases}
\begin{cases}
\det\left(\boldsymbol{u},\boldsymbol{v}\right)=\det\left(\boldsymbol{u}+s\boldsymbol{v},\boldsymbol{v}\right)\\
\det\left(\boldsymbol{u},\boldsymbol{v}\right)=\det\left(\boldsymbol{u},\boldsymbol{v}+s\boldsymbol{u}\right)
\end{cases} & \text{translation invariance}\\
\begin{cases}
\det\left(\boldsymbol{u}_{{\scriptscriptstyle 1}}+s\boldsymbol{u}_{{\scriptscriptstyle 2}},\boldsymbol{v}\right)=\det\left(\boldsymbol{u}_{{\scriptscriptstyle 1}},\boldsymbol{v}\right)+s\det\left(\boldsymbol{u}_{{\scriptscriptstyle 2}},\boldsymbol{v}\right)\\
\det\left(\boldsymbol{u},\boldsymbol{v}_{{\scriptscriptstyle 1}}+s\boldsymbol{v}_{{\scriptscriptstyle 2}}\right)=\det\left(\boldsymbol{u},\boldsymbol{v}_{{\scriptscriptstyle 1}}\right)+s\det\left(\boldsymbol{u},\boldsymbol{v}_{{\scriptscriptstyle 2}}\right)
\end{cases} & \text{linearity}
\end{cases}
\end{aligned}
$$

## determinant theorems or properties

## ellipse area

## Cramer rule geometry perspective