# Fourier analysis

## basic calculation

$$
\int_{\frac{-\tau}{2}+\psi}^{\frac{\tau}{2}+\psi}\cos\left(n\frac{2\pi}{\tau}t+\phi\right){\rm d}t=\left[\frac{\sin\left(n\frac{2\pi}{\tau}t+\phi\right)}{n\frac{2\pi}{\tau}}\right]_{\frac{-\tau}{2}+\psi}^{\frac{\tau}{2}+\psi}=0
$$

$$
\begin{aligned}
\cos\alpha\cos\beta= & \frac{\cos\left(\alpha+\beta\right)+\cos\left(\alpha-\beta\right)}{2}\\
\sin\alpha\sin\beta= & \frac{-\cos\left(\alpha+\beta\right)+\cos\left(\alpha-\beta\right)}{2}\\
\sin\alpha\cos\beta= & \frac{\sin\left(\alpha+\beta\right)+\sin\left(\alpha-\beta\right)}{2}\\
\cos\alpha\sin\beta= & \frac{\sin\left(\alpha+\beta\right)-\sin\left(\alpha-\beta\right)}{2}
\end{aligned}
$$

$$
\begin{aligned}
 & \int\cos\left(m\frac{2\pi}{\tau}t\right)\cos\left(n\frac{2\pi}{\tau}t+\phi_{n}\right){\rm d}t\\
= & \begin{cases}
\int\cos\phi_{0}{\rm d}t & m=n=0\\
\int\dfrac{\cos\left(\left(m+n\right)\frac{2\pi}{\tau}t+\phi_{n}\right)+\cos\left(\left(m-n\right)\frac{2\pi}{\tau}t-\phi_{n}\right){\rm d}t}{2} & mn\ne0
\end{cases}\\
= & \begin{cases}
t\cos\phi_{0} & m=n=0\\
\begin{cases}
\int\dfrac{\cos\left(2n\frac{2\pi}{\tau}t+\phi_{n}\right)+\cos\left(-\phi_{n}\right)}{2}{\rm d}t & m=n\\
\int\dfrac{\cos\left(\left(m+n\right)\frac{2\pi}{\tau}t+\phi_{n}\right)+\cos\left(\left(m-n\right)\frac{2\pi}{\tau}t-\phi_{n}\right)}{2}{\rm d}t & m\ne n
\end{cases} & mn\ne0
\end{cases}\\
= & \begin{cases}
t\cos\phi_{0} & m=n=0\\
\begin{cases}
\int\dfrac{\cos\left(2n\frac{2\pi}{\tau}t+\phi_{n}\right)+\cos\phi_{n}}{2}{\rm d}t & m=n\\
\int\dfrac{\cos\left(\left(m+n\right)\frac{2\pi}{\tau}t+\phi_{n}\right)+\cos\left(\left(m-n\right)\frac{2\pi}{\tau}t-\phi_{n}\right)}{2}{\rm d}t & m\ne n
\end{cases} & mn\ne0
\end{cases}\\
= & \begin{cases}
t\cos\phi_{0} & m=n=0\\
\begin{cases}
\int\dfrac{\cos\left(2n\frac{2\pi}{\tau}t+\phi_{n}\right)}{2}{\rm d}t+\frac{t\cos\phi_{n}}{2} & m=n\\
\int\dfrac{\cos\left(\left(m+n\right)\frac{2\pi}{\tau}t+\phi_{n}\right)+\cos\left(\left(m-n\right)\frac{2\pi}{\tau}t-\phi_{n}\right)}{2}{\rm d}t & m\ne n
\end{cases} & mn\ne0
\end{cases}
\end{aligned}
$$

$$
\begin{aligned}
\cos\alpha\cos\beta= & \frac{\cos\left(\alpha+\beta\right)+\cos\left(\alpha-\beta\right)}{2}\\
\sin\alpha\sin\beta= & \frac{-\cos\left(\alpha+\beta\right)+\cos\left(\alpha-\beta\right)}{2}\\
\sin\alpha\cos\beta= & \frac{\sin\left(\alpha+\beta\right)+\sin\left(\alpha-\beta\right)}{2}\\
\cos\alpha\sin\beta= & \frac{\sin\left(\alpha+\beta\right)-\sin\left(\alpha-\beta\right)}{2}
\end{aligned}
$$

$$
\begin{aligned}
 & \int_{\frac{-\tau}{2}+\psi}^{\frac{\tau}{2}+\psi}\cos\left(m\frac{2\pi}{\tau}t\right)\cos\left(n\frac{2\pi}{\tau}t+\phi_{n}\right){\rm d}t\\
= & \begin{cases}
\tau\cos\phi_{0} & m=n=0\\
\begin{cases}
\frac{\tau\cos\phi_{n}}{2} & m=n\\
0 & m\ne n
\end{cases} & mn\ne0
\end{cases}\\
= & \begin{cases}
\begin{cases}
\tau\cos\phi_{0} & n=0\\
\frac{\tau\cos\phi_{n}}{2} & n\ne0
\end{cases} & m=n\\
0 & m\ne n
\end{cases}
\end{aligned}
$$

$$
\begin{aligned}
 & \frac{2}{\tau\cos\phi_{n}}\int_{\frac{-\tau}{2}+\psi}^{\frac{\tau}{2}+\psi}\cos\left(m\frac{2\pi}{\tau}t\right)\cos\left(n\frac{2\pi}{\tau}t+\phi_{n}\right){\rm d}t\\
= & \begin{cases}
\begin{cases}
2 & n=0\\
1 & n\ne0
\end{cases} & m=n\\
0 & m\ne n
\end{cases}
\end{aligned}
$$

$$
\begin{aligned}
 & \int_{\frac{-\tau}{2}+\psi}^{\frac{\tau}{2}+\psi}\sin\left(m\frac{2\pi}{\tau}t\right)\cos\left(n\frac{2\pi}{\tau}t+\phi_{n}\right){\rm d}t\\
= & \begin{cases}
0 & m=n\\
0 & m\ne n
\end{cases}
\end{aligned}
$$

$$
\begin{aligned}
 & \int_{\frac{-\tau}{2}+\psi}^{\frac{\tau}{2}+\psi}\cos\left(m\frac{2\pi}{\tau}t\right)\sin\left(n\frac{2\pi}{\tau}t+\phi_{n}\right){\rm d}t\\
= & \begin{cases}
0 & m=n\\
0 & m\ne n
\end{cases}
\end{aligned}
$$

***

$$
\begin{aligned}
\frac{2}{\tau\cos\phi_{n}}\int_{\frac{-\tau}{2}+\psi}^{\frac{\tau}{2}+\psi}\cos\left(m\frac{2\pi}{\tau}t\right)\cos\left(n\frac{2\pi}{\tau}t+\phi_{n}\right){\rm d}t= & \begin{cases}
\begin{cases}
2 & n=0\\
1 & n\ne0
\end{cases} & m=n\\
0 & m\ne n
\end{cases}\\
\frac{2}{\tau\cos\phi_{n}}\int_{\frac{-\tau}{2}+\psi}^{\frac{\tau}{2}+\psi}\sin\left(m\frac{2\pi}{\tau}t\right)\sin\left(n\frac{2\pi}{\tau}t+\phi_{n}\right){\rm d}t= & \begin{cases}
1 & m=n\ne0\\
0 & \neg\left(m=n\ne0\right)
\end{cases}\\
\int_{\frac{-\tau}{2}+\psi}^{\frac{\tau}{2}+\psi}\sin\left(m\frac{2\pi}{\tau}t\right)\cos\left(n\frac{2\pi}{\tau}t+\phi_{n}\right){\rm d}t= & \begin{cases}
0 & m=n\\
0 & m\ne n
\end{cases}\\
\int_{\frac{-\tau}{2}+\psi}^{\frac{\tau}{2}+\psi}\cos\left(m\frac{2\pi}{\tau}t\right)\sin\left(n\frac{2\pi}{\tau}t+\phi_{n}\right){\rm d}t= & \begin{cases}
0 & m=n\\
0 & m\ne n
\end{cases}
\end{aligned}
$$

***

## Simon Xu

### DFT = discrete Fourier transform

::: {show-in="html"}
<iframe width=500 height=300 frameborder="0" allowfullscreen src="https://www.youtube.com/embed/mkGsMWi_j4Q"></iframe>
:::

### FFT = fast Fourier transform

::: {show-in="html"}
<iframe width=500 height=300 frameborder="0" allowfullscreen src="https://www.youtube.com/embed/htCj9exbGo0"></iframe>
:::

### wavelet

::: {show-in="html"}
<iframe width=500 height=300 frameborder="0" allowfullscreen src="https://www.youtube.com/embed/ZnmvUCtUAEE"></iframe>
:::