# Feynman method

## Feynman method of differentiation / derivative

::: {show-in="html"}
<iframe width=500 height=300 frameborder="0" allowfullscreen src="https://player.bilibili.com/player.html?bvid=BV1hG411Z7Cb&autoplay=0"></iframe>
:::


::: {show-in="html"}
分式微分不是難而是煩
:::

::: {show-in="pdf"}
\begin{CJK}{UTF8}{bsmi}
分式微分不是難而是煩
\end{CJK}
:::



### principle

```{theorem}
Feynman method of differentiation / derivative
```

$$
\begin{array}{c}
f\left(t\right)=k\left[u\left(t\right)\right]^{a}\left[v\left(t\right)\right]^{b}\left[w\left(t\right)\right]^{c}\cdots\\
\Downarrow\\
f^{\prime}\left(t\right)=f\left(t\right)\left[a\dfrac{u^{\prime}\left(t\right)}{u\left(t\right)}+b\dfrac{v^{\prime}\left(t\right)}{v\left(t\right)}+c\dfrac{w^{\prime}\left(t\right)}{w\left(t\right)}+\cdots\right]
\end{array}
$$

Proof:

$$
f\left(t\right)=k\left[u\left(t\right)\right]^{a}\left[v\left(t\right)\right]^{b}\left[w\left(t\right)\right]^{c}\cdots
$$

$$
f=ku^{a}v^{b}w^{c}\cdots=k\cdot u^{a}\cdot v^{b}\cdot w^{c}\cdot\cdots
$$

$$
\begin{aligned}
f= & ku^{a}v^{b}w^{c}\cdots=k\cdot u^{a}\cdot v^{b}\cdot w^{c}\cdot\cdots\\
\ln f= & \ln\left(ku^{a}v^{b}w^{c}\cdots\right)=\ln k+\ln u^{a}+\ln v^{b}+\ln w^{c}+\cdots\\
= & \ln k+a\ln u+b\ln v+c\ln w+\cdots\\
\dfrac{\mathrm{d}}{\mathrm{d}t}\ln f= & \dfrac{\mathrm{d}}{\mathrm{d}t}\left(\ln k+a\ln u+b\ln v+c\ln w+\cdots\right)\\
\dfrac{\dfrac{\mathrm{d}}{\mathrm{d}t}f}{f}= & 0+\dfrac{\mathrm{d}}{\mathrm{d}t}\left(a\ln u\right)+\dfrac{\mathrm{d}}{\mathrm{d}t}\left(b\ln v\right)+\dfrac{\mathrm{d}}{\mathrm{d}t}\left(c\ln w\right)+\cdots\\
= & a\dfrac{\mathrm{d}}{\mathrm{d}t}\ln u+b\dfrac{\mathrm{d}}{\mathrm{d}t}\ln v+c\dfrac{\mathrm{d}}{\mathrm{d}t}\ln w+\cdots\\
= & a\dfrac{\dfrac{\mathrm{d}}{\mathrm{d}t}u}{u}+b\dfrac{\dfrac{\mathrm{d}}{\mathrm{d}t}v}{v}+c\dfrac{\dfrac{\mathrm{d}}{\mathrm{d}t}w}{w}+\cdots\\
\dfrac{f^{\prime}}{f}= & a\dfrac{u^{\prime}}{u}+b\dfrac{v^{\prime}}{v}+c\dfrac{w^{\prime}}{w}+\cdots\\
f^{\prime}= & f\left(a\dfrac{u^{\prime}}{u}+b\dfrac{v^{\prime}}{v}+c\dfrac{w^{\prime}}{w}+\cdots\right)\\
f^{\prime}\left(t\right)= & f\left(t\right)\left[a\dfrac{u^{\prime}\left(t\right)}{u\left(t\right)}+b\dfrac{v^{\prime}\left(t\right)}{v\left(t\right)}+c\dfrac{w^{\prime}\left(t\right)}{w\left(t\right)}+\cdots\right]
\end{aligned}
$$

$$
\tag*{$\Box$}
$$

### examples

$f\left(x\right)=x^{x}$

$$
\left(x^{x}\right)^{\prime}=x^{x}+x^{x}\ln x
$$

$$
\begin{aligned}
f\left(x\right)= & x^{x}\\
\ln f\left(x\right)= & x\ln x\\
\dfrac{\mathrm{d}}{\mathrm{d}x}\ln f\left(x\right)= & \dfrac{\mathrm{d}}{\mathrm{d}x}\left[x\ln x\right]\\
\dfrac{f^{\prime}\left(x\right)}{f\left(x\right)}= & \left[x\ln x\right]^{\prime}\\
f^{\prime}\left(x\right)= & f\left(x\right)\left[x\ln x\right]^{\prime}=x^{x}\left[\left(x\right)^{\prime}\ln x+x\left(\ln x\right)^{\prime}\right]\\
= & x^{x}\left[1\ln x+x\dfrac{1}{x}\right]=x^{x}\left[\ln x+1\right]=x^{x}\left[1+\ln x\right]\\
= & x^{x}+x^{x}\ln x
\end{aligned}
$$

$$
\tag*{$\Box$}
$$

***

$\Delta\left(\dfrac{1}{r}\right)=\boldsymbol{\nabla}^{2}\left(\dfrac{1}{\sqrt{\boldsymbol{r}^{2}}}\right)=\boldsymbol{\nabla}\cdot\boldsymbol{\nabla}\left(\dfrac{1}{\sqrt{\boldsymbol{r}\cdot\boldsymbol{r}}}\right)=\boldsymbol{\nabla}\cdot\left(\dfrac{\partial}{\partial x},\dfrac{\partial}{\partial y},\dfrac{\partial}{\partial z}\right)\left(\dfrac{1}{\sqrt{x^{2}+y^{2}+z^{2}}}\right)$

$$
\dfrac{\partial}{\partial x}\dfrac{1}{\sqrt{x^{2}+y^{2}+z^{2}}}
$$

$$
\begin{aligned}
 & \dfrac{\partial}{\partial x}\dfrac{1}{\sqrt{x^{2}+y^{2}+z^{2}}}=\dfrac{\partial}{\partial x}\left[\left(x^{2}+y^{2}+z^{2}\right)^{\frac{-1}{2}}\right]\\
= & \left(x^{2}+y^{2}+z^{2}\right)^{\frac{-1}{2}}\left[\frac{-1}{2}\dfrac{2x}{x^{2}+y^{2}+z^{2}}\right]\\
= & \dfrac{-x}{\left(x^{2}+y^{2}+z^{2}\right)^{\frac{-3}{2}}}
\end{aligned}
$$

$$
\boldsymbol{\nabla}\left(\dfrac{1}{r}\right)=\boldsymbol{\nabla}\left(\dfrac{1}{\sqrt{\boldsymbol{r}\cdot\boldsymbol{r}}}\right)=\left(\dfrac{\partial}{\partial x},\dfrac{\partial}{\partial y},\dfrac{\partial}{\partial z}\right)\left(\dfrac{1}{\sqrt{x^{2}+y^{2}+z^{2}}}\right)=\left(\dfrac{-x}{\left(x^{2}+y^{2}+z^{2}\right)^{\frac{3}{2}}},\dfrac{-y}{\left(x^{2}+y^{2}+z^{2}\right)^{\frac{3}{2}}},\dfrac{-z}{\left(x^{2}+y^{2}+z^{2}\right)^{\frac{3}{2}}}\right)
$$

$$
\begin{aligned}
\boldsymbol{\nabla}\cdot\boldsymbol{\nabla}\left(\dfrac{1}{r}\right)= & \boldsymbol{\nabla}\cdot\left(\dfrac{-x}{\left(x^{2}+y^{2}+z^{2}\right)^{\frac{3}{2}}},\dfrac{-y}{\left(x^{2}+y^{2}+z^{2}\right)^{\frac{3}{2}}},\dfrac{-z}{\left(x^{2}+y^{2}+z^{2}\right)^{\frac{3}{2}}}\right)\\
= & \dfrac{\partial}{\partial x}\dfrac{-x}{\left(x^{2}+y^{2}+z^{2}+\epsilon^{2}\right)^{\frac{3}{2}}}+\dfrac{\partial}{\partial y}\dfrac{-y}{\left(x^{2}+y^{2}+z^{2}+\epsilon^{2}\right)^{\frac{3}{2}}}+\dfrac{\partial}{\partial z}\dfrac{-z}{\left(x^{2}+y^{2}+z^{2}+\epsilon^{2}\right)^{\frac{3}{2}}}
\end{aligned}
$$

$$
\dfrac{\partial}{\partial x}\dfrac{-x}{\left(x^{2}+y^{2}+z^{2}+\epsilon^{2}\right)^{\frac{3}{2}}}
$$

$$
\begin{aligned}
 & \dfrac{\partial}{\partial x}\dfrac{-x}{\left(x^{2}+y^{2}+z^{2}\right)^{\frac{3}{2}}}\\
= & \dfrac{-x}{\left(x^{2}+y^{2}+z^{2}\right)^{\frac{3}{2}}}\left[1\cdot\dfrac{1}{x}+\dfrac{-3}{2}\dfrac{2x}{x^{2}+y^{2}+z^{2}}\right]\\
= & \dfrac{-1}{\left(x^{2}+y^{2}+z^{2}\right)^{\frac{3}{2}}}+\dfrac{3x^{2}}{\left(x^{2}+y^{2}+z^{2}\right)^{\frac{5}{2}}}\\
= & \dfrac{-\left(x^{2}+y^{2}+z^{2}\right)+3x^{2}}{\left(x^{2}+y^{2}+z^{2}\right)^{\frac{5}{2}}}=\dfrac{2x^{2}-y^{2}-z^{2}}{\left(x^{2}+y^{2}+z^{2}\right)^{\frac{5}{2}}}
\end{aligned}
$$

$$
\begin{aligned}
\boldsymbol{\nabla}\cdot\boldsymbol{\nabla}\left(\dfrac{1}{r}\right)= & \dfrac{\partial}{\partial x}\dfrac{-x}{\left(x^{2}+y^{2}+z^{2}+\epsilon^{2}\right)^{\frac{3}{2}}}+\dfrac{\partial}{\partial y}\dfrac{-y}{\left(x^{2}+y^{2}+z^{2}+\epsilon^{2}\right)^{\frac{3}{2}}}+\dfrac{\partial}{\partial z}\dfrac{-z}{\left(x^{2}+y^{2}+z^{2}+\epsilon^{2}\right)^{\frac{3}{2}}}\\
= & \dfrac{+2x^{2}-y^{2}-z^{2}}{\left(x^{2}+y^{2}+z^{2}\right)^{\frac{5}{2}}}+\dfrac{-x^{2}+2y^{2}-z^{2}}{\left(x^{2}+y^{2}+z^{2}\right)^{\frac{5}{2}}}+\dfrac{-x^{2}-y^{2}+2z^{2}}{\left(x^{2}+y^{2}+z^{2}\right)^{\frac{5}{2}}}=0
\end{aligned}
$$

$$
\Delta\left(\dfrac{1}{r}\right)=\boldsymbol{\nabla}\cdot\boldsymbol{\nabla}\left(\dfrac{1}{r}\right)=0
$$

$$
\tag*{$\Box$}
$$

***

$\dfrac{6\left(1+2t^{2}\right)\left(t^{3}-t\right)^{2}}{\sqrt{t+5t^{2}}\left(4t\right)^{\frac{3}{2}}}+\dfrac{\sqrt{1+2t}}{t+\sqrt{1+t^{2}}}$

$$
\dfrac{\mathrm{d}}{\mathrm{d}t}\left[\dfrac{6\left(1+2t^{2}\right)\left(t^{3}-t\right)^{2}}{\sqrt{t+5t^{2}}\left(4t\right)^{\frac{3}{2}}}+\dfrac{\sqrt{1+2t}}{t+\sqrt{1+t^{2}}}\right]
$$

***

$$
\dfrac{\mathrm{d}}{\mathrm{d}t}\left[\dfrac{6\left(1+2t^{2}\right)\left(t^{3}-t\right)^{2}}{\sqrt{t+5t^{2}}\left(4t\right)^{\frac{3}{2}}}\right]
$$

$$
\begin{aligned}
 & \dfrac{\mathrm{d}}{\mathrm{d}t}\left[\dfrac{6\left(1+2t^{2}\right)\left(t^{3}-t\right)^{2}}{\sqrt{t+5t^{2}}\left(4t\right)^{\frac{3}{2}}}\right]\\
= & \dfrac{6\left(1+2t^{2}\right)\left(t^{3}-t\right)^{2}}{\sqrt{t+5t^{2}}\left(4t\right)^{\frac{3}{2}}}\cdot[\\
= & \dfrac{6\left[1+2t^{2}\right]\left(t^{3}-t\right)^{2}}{\sqrt{t+5t^{2}}\left(4t\right)^{\frac{3}{2}}}\cdot[1\cdot\dfrac{1}{1+2t^{2}}\cdot4t,\left[1+2t^{2}\right]\rightarrow\begin{cases}
\text{exponential}: & 1\\
\text{linear to denominator}: & \dfrac{1}{1+2t^{2}}\\
\text{differentiation} & 4t
\end{cases}\\
= & \dfrac{6\left(1+2t^{2}\right)\left[\left(t^{3}-t\right)^{2}\right]}{\sqrt{t+5t^{2}}\left(4t\right)^{\frac{3}{2}}}\cdot[\dfrac{4t}{1+2t^{2}}+2\cdot\dfrac{1}{t^{3}-t}\cdot\left(3t^{2}-1\right)\\
 & ,\left[\left(t^{3}-t\right)^{2}\right]\rightarrow\begin{cases}
\text{exponential}: & 2\\
\text{linear to denominator}: & \dfrac{1}{t^{3}-t}\\
\text{differentiation} & 3t^{2}-1
\end{cases}\\
= & \dfrac{6\left(1+2t^{2}\right)\left(t^{3}-t\right)^{2}}{\left[\sqrt{t+5t^{2}}\right]\left(4t\right)^{\frac{3}{2}}}\cdot[\dfrac{4t}{1+2t^{2}}+\dfrac{6t^{2}-2}{t^{3}-t}+\dfrac{-1}{2}\cdot\dfrac{1}{t+5t^{2}}\cdot\left(1+10t\right)\\
 & ,\left[\sqrt{t+5t^{2}}\right]\rightarrow\begin{cases}
\text{exponential}: & \dfrac{-1}{2}\\
\text{linear to denominator}: & \dfrac{1}{t+5t^{2}}\\
\text{differentiation} & 1+10t
\end{cases}\\
= & \dfrac{6\left(1+2t^{2}\right)\left(t^{3}-t\right)^{2}}{\sqrt{t+5t^{2}}\left[\left(4t\right)^{\frac{3}{2}}\right]}\cdot\left[\dfrac{4t}{1+2t^{2}}+\dfrac{6t^{2}-2}{t^{3}-t}-\dfrac{1+10t}{2t+10t^{2}}+\dfrac{-3}{2}\cdot\dfrac{1}{4t}\cdot4\right]\\
 & ,\left[\left(4t\right)^{\frac{3}{2}}\right]\rightarrow\begin{cases}
\text{exponential}: & \dfrac{-3}{2}\\
\text{linear to denominator}: & \dfrac{1}{4t}\\
\text{differentiation} & 4
\end{cases}\\
= & \dfrac{6\left(1+2t^{2}\right)\left(t^{3}-t\right)^{2}}{\sqrt{t+5t^{2}}\left(4t\right)^{\frac{3}{2}}}\left[\dfrac{4t}{1+2t^{2}}+\dfrac{6t^{2}-2}{t^{3}-t}-\dfrac{1+10t}{2t+10t^{2}}-\dfrac{3}{2t}\right]
\end{aligned}
$$

***

$$
\dfrac{\mathrm{d}}{\mathrm{d}t}\left[\dfrac{\sqrt{1+2t}}{t+\sqrt{1+t^{2}}}\right]
$$

$$
\begin{aligned}
 & \dfrac{\mathrm{d}}{\mathrm{d}t}\left[\dfrac{\sqrt{1+2t}}{t+\sqrt{1+t^{2}}}\right]\\
= & \dfrac{\sqrt{1+2t}}{t+\left[\sqrt{1+t^{2}}\right]}\left[\dfrac{1}{2}\dfrac{2}{1+2t}+\left(-1\right)\dfrac{1+\left[\frac{1}{2}\frac{2t}{\sqrt{1+t^{2}}}\right]}{t+\sqrt{1+t^{2}}}\right]
\end{aligned}
$$

$$
\tag*{$\Box$}
$$

## Feynman method of integration / integral

## path integral

https://www.youtube.com/watch?v=Sp5SvdDh2u8

https://en.wikipedia.org/wiki/Path_integral_formulation

https://www.youtube.com/watch?v=7yjv-gLHFqg