# group theory

::: {show-in="html"}
<iframe width=500 height=300 frameborder="0" allowfullscreen src="https://player.bilibili.com/player.html?bvid=BV1hm4y1v75R&autoplay=0"></iframe>
:::

## complex group representation

$\mathbb{C}\rightarrow\mathcal{M}_{2\times2}\left(\mathbb{R}\right)$

$$
1\leftrightarrow\begin{pmatrix}1 & 0\\
0 & 1
\end{pmatrix}=I_{2}=I
$$

$$
\begin{aligned}
c_{{\scriptscriptstyle 1}}\begin{pmatrix}1 & 0\\
0 & 1
\end{pmatrix}+c_{{\scriptscriptstyle 2}}\begin{pmatrix}a & b\\
c & d
\end{pmatrix}= & x\begin{pmatrix}1 & 0\\
0 & 1
\end{pmatrix}+y\begin{pmatrix}a & b\\
c & d
\end{pmatrix},\left\langle a,b,c,d\right\rangle \in\mathbb{R}^{4}\\
= & xI+yJ,J=\begin{pmatrix}a & b\\
c & d
\end{pmatrix}\in\mathcal{M}_{2\times2}\left(\mathbb{R}\right),\left\langle x,y\right\rangle \in\mathbb{R}^{2}
\end{aligned}
$$

***

$$
J^{2}=-I
$$

***

$$
\begin{aligned}
J^{2}= & -I\\
\begin{pmatrix}a^{2}+bc & ab+bd\\
ca+cd & cb+d^{2}
\end{pmatrix}=\begin{pmatrix}a & b\\
c & d
\end{pmatrix}\begin{pmatrix}a & b\\
c & d
\end{pmatrix}= & -\begin{pmatrix}1 & 0\\
0 & 1
\end{pmatrix}=\begin{pmatrix}-1 & 0\\
0 & -1
\end{pmatrix}\\
\begin{cases}
a^{2}+bc=-1 & b=0\Rightarrow a^{2}=-1\Rightarrow\Leftarrow a\in\mathbb{R}\Rightarrow b\ne0\\
ab+bd=0 & \left(b=0\right)\vee\left(a=-d\right)\overset{b\ne0}{\Rightarrow}a=-d\\
ca+cd=0\\
cb+d^{2}=-1 & a^{2}=d^{2}\Rightarrow\left(a=d\right)\vee\left(a=-d\right)
\end{cases} & \overset{\text{if }a=d}{\Rightarrow}\begin{cases}
a=d\\
a=-d
\end{cases}\\
 & \Rightarrow a=d=0\Rightarrow bc=-1
\end{aligned}
$$
$$
J=\begin{pmatrix}a & b\\
c & d
\end{pmatrix}=\begin{pmatrix}a & b\\
\dfrac{-a^{2}-1}{b} & -a
\end{pmatrix}=J\left(a,b\right),b\ne0
$$

$$
\begin{aligned}
J\left(a,b\right)=\begin{pmatrix}a & b\\
\dfrac{-a^{2}-1}{b} & -a
\end{pmatrix},b\ne0
\end{aligned}
$$

***

$$
J\left(a=1,b\right)=\begin{pmatrix}1 & b\\
\dfrac{-2}{b} & -1
\end{pmatrix}\Rightarrow J^{2}\left(a=1,b\right)=\begin{pmatrix}-1 & 0\\
0 & -1
\end{pmatrix}=-I
$$

$$
\begin{aligned}
xI+yJ\left(a=1,b\right)=\begin{pmatrix}x+y & yb\\
y\cdot\dfrac{-2}{b} & x-y
\end{pmatrix}
\end{aligned}
$$

***

$$
J\left(a=0,b\right)=\begin{pmatrix}0 & b\\
\dfrac{-1}{b} & 0
\end{pmatrix}
$$

***

$$
J\left(a=0,b=1\right)=\begin{pmatrix}0 & 1\\
-1 & 0
\end{pmatrix}
$$

***

$$
\begin{aligned}
J\left(a=0,b=-1\right)= & \begin{pmatrix}0 & -1\\
1 & 0
\end{pmatrix}=-\begin{pmatrix}0 & 1\\
-1 & 0
\end{pmatrix}=-J\left(a=0,b=1\right)\\
\Rightarrow J^{2}\left(a=0,b=-1\right)= & \begin{pmatrix}0 & -1\\
1 & 0
\end{pmatrix}\begin{pmatrix}0 & -1\\
1 & 0
\end{pmatrix}=\begin{pmatrix}-1 & 0\\
0 & -1
\end{pmatrix}=-I
\end{aligned}
$$

$$
\begin{aligned}
J=J\left(a=0,b=-1\right)= & \begin{pmatrix}0 & -1\\
1 & 0
\end{pmatrix}\\
\Rightarrow & \begin{cases}
1\leftrightarrow I=\begin{pmatrix}1 & 0\\
0 & 1
\end{pmatrix}\\
\mathrm{i}\leftrightarrow J=\begin{pmatrix}0 & -1\\
1 & 0
\end{pmatrix}
\end{cases}\\
\Rightarrow x+y\mathrm{i}\leftrightarrow & xI+yJ\\
= & x\begin{pmatrix}1 & 0\\
0 & 1
\end{pmatrix}+y\begin{pmatrix}0 & -1\\
1 & 0
\end{pmatrix}=\begin{pmatrix}x & -y\\
y & x
\end{pmatrix}
\end{aligned}
$$

$$
x+y\mathrm{i}\leftrightarrow\begin{pmatrix}x & -y\\
y & x
\end{pmatrix}=xI+yJ
$$

$$
\mathbb{C}\rightarrow\mathcal{M}_{2\times2}\left(\mathbb{R}\right)
$$

### Euler formula proved by complex group representation

::: {show-in="html"}
<iframe width=500 height=300 frameborder="0" allowfullscreen src="https://player.bilibili.com/player.html?bvid=BV1mM4y1J79a&autoplay=0"></iframe>
:::

$$
\begin{aligned}
\begin{pmatrix}x^{\prime}\\
y^{\prime}
\end{pmatrix}= & \begin{pmatrix}\cos\theta & -\sin\theta\\
\sin\theta & \cos\theta
\end{pmatrix}\begin{pmatrix}x\\
y
\end{pmatrix}=R_{{\scriptscriptstyle \theta}}\begin{pmatrix}x\\
y
\end{pmatrix}\\
= & \begin{pmatrix}\cos n\frac{\theta}{n} & -\sin n\frac{\theta}{n}\\
\sin n\frac{\theta}{n} & \cos n\frac{\theta}{n}
\end{pmatrix}\begin{pmatrix}x\\
y
\end{pmatrix}=\begin{pmatrix}\cos\frac{\theta}{n} & -\sin\frac{\theta}{n}\\
\sin\frac{\theta}{n} & \cos\frac{\theta}{n}
\end{pmatrix}^{n}\begin{pmatrix}x\\
y
\end{pmatrix}=R_{{\scriptscriptstyle \frac{\theta}{n}}}^{n}\begin{pmatrix}x\\
y
\end{pmatrix}
\end{aligned}
$$

$$
\begin{aligned}
\lim_{n\rightarrow\infty}R_{{\scriptscriptstyle \frac{\theta}{n}}}= & \lim_{n\rightarrow\infty}\begin{pmatrix}\cos\frac{\theta}{n} & -\sin\frac{\theta}{n}\\
\sin\frac{\theta}{n} & \cos\frac{\theta}{n}
\end{pmatrix}=\begin{pmatrix}1 & -\frac{\theta}{n}\\
\frac{\theta}{n} & 1
\end{pmatrix}\\
= & \begin{pmatrix}1 & 0\\
0 & 1
\end{pmatrix}+\dfrac{\theta}{n}\begin{pmatrix}0 & -1\\
1 & 0
\end{pmatrix}=\begin{pmatrix}1 & 0\\
0 & 1
\end{pmatrix}+\dfrac{\theta}{n}\begin{pmatrix}\cos\frac{\pi}{2} & -\sin\frac{\pi}{2}\\
\sin\frac{\pi}{2} & \cos\frac{\pi}{2}
\end{pmatrix}=I+\dfrac{\theta}{n}R_{{\scriptscriptstyle \frac{\pi}{2}}}
\end{aligned}
$$

$$
\begin{aligned}
\begin{pmatrix}x^{\prime}\\
y^{\prime}
\end{pmatrix}=\lim_{n\rightarrow\infty}\begin{pmatrix}x^{\prime}\\
y^{\prime}
\end{pmatrix}= & \lim_{n\rightarrow\infty}R_{{\scriptscriptstyle \frac{\theta}{n}}}^{n}\begin{pmatrix}x\\
y
\end{pmatrix}=\left(\lim_{n\rightarrow\infty}R_{{\scriptscriptstyle \frac{\theta}{n}}}^{n}\right)\left(\lim_{n\rightarrow\infty}\begin{pmatrix}x\\
y
\end{pmatrix}\right)=\left(\lim_{n\rightarrow\infty}R_{{\scriptscriptstyle \frac{\theta}{n}}}^{n}\right)\begin{pmatrix}x\\
y
\end{pmatrix}\\
= & \lim_{n\rightarrow\infty}\left(\lim_{n\rightarrow\infty}R_{{\scriptscriptstyle \frac{\theta}{n}}}\right)^{n}\begin{pmatrix}x\\
y
\end{pmatrix}=\lim_{n\rightarrow\infty}\left(I+\dfrac{\theta}{n}R_{{\scriptscriptstyle \frac{\pi}{2}}}\right)^{n}\begin{pmatrix}x\\
y
\end{pmatrix}\\
= & \lim_{n\rightarrow\infty}\left(I+\dfrac{\theta}{n}\begin{pmatrix}0 & -1\\
1 & 0
\end{pmatrix}\right)^{n}\begin{pmatrix}x\\
y
\end{pmatrix}=\lim_{n\rightarrow\infty}\left(I+\dfrac{\theta J}{n}\right)^{n}\begin{pmatrix}x\\
y
\end{pmatrix},J=\begin{pmatrix}0 & -1\\
1 & 0
\end{pmatrix}\\
= & \mathrm{e}^{J\theta}\begin{pmatrix}x\\
y
\end{pmatrix}
\end{aligned}
$$

$$
\begin{aligned}
 & \begin{cases}
\begin{pmatrix}x^{\prime}\\
y^{\prime}
\end{pmatrix}=\begin{pmatrix}\cos\theta & -\sin\theta\\
\sin\theta & \cos\theta
\end{pmatrix}\begin{pmatrix}x\\
y
\end{pmatrix}\\
\begin{pmatrix}x^{\prime}\\
y^{\prime}
\end{pmatrix}=\mathrm{e}^{J\theta}\begin{pmatrix}x\\
y
\end{pmatrix}
\end{cases}\\
\Rightarrow & \mathrm{e}^{J\theta}=\begin{pmatrix}\cos\theta & -\sin\theta\\
\sin\theta & \cos\theta
\end{pmatrix}\overset{x+y\mathrm{i}\leftrightarrow\begin{pmatrix}x & -y\\
y & x
\end{pmatrix}=xI+yJ}{\Rightarrow}\mathrm{e}^{\mathrm{i}\theta}=\cos\theta+\mathrm{i}\sin\theta
\end{aligned}
$$

$$
\ \tag*{$\Box$}
$$
### Lagrange identity

https://en.wikipedia.org/wiki/Lagrange%27s_identity

generalization of [Brahmagupta–Fibonacci identity](https://en.wikipedia.org/wiki/Lagrange's_identity)

specialization of [Binet–Cauchy identity](https://en.wikipedia.org/wiki/Binet–Cauchy_identity)

## quaternion group representation

https://groupprops.subwiki.org/wiki/Linear_representation_theory_of_quaternion_group#Two-dimensional_irreducible_representation_over_a_splitting_field

$$
\begin{aligned}
 & q=a+b\mathrm{i}+c\mathrm{j}+d\mathrm{k}=a+\mathrm{i}b+\mathrm{j}c+\mathrm{k}d,\begin{cases}
q\in\mathbb{H}\\
a,b,c,d\in\mathbb{R} & \Leftrightarrow\left\langle a,b,c,d\right\rangle \in\mathbb{R}^{4}
\end{cases}\\
= & w=t+x\mathrm{i}+y\mathrm{j}+z\mathrm{k}=t+\mathrm{i}x+\mathrm{j}y+\mathrm{k}z,\begin{cases}
w\in\mathbb{H}\\
t,x,y,z\in\mathbb{R} & \Leftrightarrow\left\langle t,x,y,z\right\rangle \in\mathbb{R}^{4}
\end{cases}\\
= & a1+b\mathrm{i}+c\mathrm{j}+d\mathrm{k}=t1+x\mathrm{i}+y\mathrm{j}+z\mathrm{k}=x_{{\scriptscriptstyle 0}}1+\boldsymbol{e}_{{\scriptscriptstyle i}}x_{{\scriptscriptstyle i}}
\end{aligned}
$$

### $\mathbb{H}\rightarrow\mathcal{M}_{2\times2}\left(\mathbb{C}\right)$

$$
1=\begin{pmatrix}1 & 0\\
0 & 1
\end{pmatrix}=1_{2}=1
$$

$$
\begin{aligned}
\boldsymbol{e}= & \begin{pmatrix}a & b\\
c & d
\end{pmatrix}=\begin{pmatrix}a & b\\
\dfrac{-a^{2}-1}{b} & -a
\end{pmatrix}\\
= & \begin{cases}
\begin{pmatrix}a & b\\
\dfrac{-a^{2}-1}{b} & -a
\end{pmatrix}=\begin{pmatrix}0 & b\\
\dfrac{-1}{b} & 0
\end{pmatrix}=\begin{pmatrix}0 & \beta\\
-\beta & 0
\end{pmatrix}\Rightarrow\boldsymbol{e}_{{\scriptscriptstyle 2}}=J=\begin{pmatrix}0 & -1\\
1 & 0
\end{pmatrix}=\mathrm{j} & a=0\\
\begin{pmatrix}a & b\\
\dfrac{-a^{2}-1}{b} & -a
\end{pmatrix}=\begin{pmatrix}\alpha & \beta\\
\beta & -\alpha
\end{pmatrix} & a\ne0
\end{cases}
\end{aligned}
$$

$$
\begin{aligned}
\begin{pmatrix}\alpha^{2}+\beta^{2} & 0\\
0 & \beta^{2}+\alpha^{2}
\end{pmatrix}=\begin{pmatrix}\alpha & \beta\\
\beta & -\alpha
\end{pmatrix}\begin{pmatrix}\alpha & \beta\\
\beta & -\alpha
\end{pmatrix}=\boldsymbol{e}^{2}= & -1=-\begin{pmatrix}1 & 0\\
0 & 1
\end{pmatrix}=\begin{pmatrix}-1 & 0\\
0 & -1
\end{pmatrix}\\
\Downarrow\\
\alpha^{2}+\beta^{2}= & -1\Leftrightarrow\beta^{2}+\alpha^{2}=-1
\end{aligned}
$$

$$
\alpha^{2}+\beta^{2}=-1\Rightarrow\left\langle \alpha,\beta\right\rangle \notin\mathbb{R}^{2}\Rightarrow\Leftarrow\left\langle \alpha,\beta\right\rangle \in\mathbb{R}^{2}\Rightarrow\alpha^{2}+\beta^{2}\ge0
$$

> quaternion group has no irreducible two-dimensional representation over the reals ^[https://groupprops.subwiki.org/wiki/Linear_representation_theory_of_quaternion_group#Four-dimensional_irreducible_representation_over_a_non-splitting_field]

$$
\left\langle \alpha,\beta\right\rangle \in\mathbb{C}^{2}-\mathbb{R}^{2}
$$

$$
\alpha^{2}+\beta^{2}=-1=\beta^{2}+\alpha^{2}
$$

$$
\begin{pmatrix}\beta & \alpha\\
\alpha & -\beta
\end{pmatrix}\begin{pmatrix}\beta & \alpha\\
\alpha & -\beta
\end{pmatrix}=\begin{pmatrix}\beta^{2}+\alpha^{2} & 0\\
0 & \alpha^{2}+\beta^{2}
\end{pmatrix}=\begin{pmatrix}-1 & 0\\
0 & -1
\end{pmatrix}=-\begin{pmatrix}1 & 0\\
0 & 1
\end{pmatrix}=-1
$$

$$
1=\begin{pmatrix}1 & 0\\
0 & 1
\end{pmatrix},\boldsymbol{e}_{{\scriptscriptstyle 1}}=\begin{pmatrix}\alpha & \beta\\
\beta & -\alpha
\end{pmatrix},\boldsymbol{e}_{{\scriptscriptstyle 2}}=\begin{pmatrix}0 & -1\\
1 & 0
\end{pmatrix}
$$

$$
1=\begin{pmatrix}1 & 0\\
0 & 1
\end{pmatrix},\mathrm{i}=\begin{pmatrix}\alpha & \beta\\
\beta & -\alpha
\end{pmatrix},\mathrm{j}=\begin{pmatrix}0 & -1\\
1 & 0
\end{pmatrix}
$$

$$
\mathrm{i}\mathrm{j}=\begin{pmatrix}\alpha & \beta\\
\beta & -\alpha
\end{pmatrix}\begin{pmatrix}0 & -1\\
1 & 0
\end{pmatrix}=\begin{pmatrix}\beta & -\alpha\\
-\alpha & -\beta
\end{pmatrix}=-\begin{pmatrix}\beta & \alpha\\
\alpha & -\beta
\end{pmatrix}
$$

$$
1=\begin{pmatrix}1 & 0\\
0 & 1
\end{pmatrix},\boldsymbol{e}_{{\scriptscriptstyle 1}}=\begin{pmatrix}\alpha & \beta\\
\beta & -\alpha
\end{pmatrix},\boldsymbol{e}_{{\scriptscriptstyle 2}}=\begin{pmatrix}0 & -1\\
1 & 0
\end{pmatrix},\boldsymbol{e}_{{\scriptscriptstyle 3}}=\begin{pmatrix}\beta & -\alpha\\
-\alpha & -\beta
\end{pmatrix}
$$
$$
1=\begin{pmatrix}1 & 0\\
0 & 1
\end{pmatrix},\mathrm{i}=\begin{pmatrix}\alpha & \beta\\
\beta & -\alpha
\end{pmatrix},\mathrm{j}=\begin{pmatrix}0 & -1\\
1 & 0
\end{pmatrix},\mathrm{k}=\begin{pmatrix}\beta & -\alpha\\
-\alpha & -\beta
\end{pmatrix}
$$

$$
\mathrm{j}\mathrm{k}=\begin{pmatrix}0 & -1\\
1 & 0
\end{pmatrix}\begin{pmatrix}\beta & -\alpha\\
-\alpha & -\beta
\end{pmatrix}=\begin{pmatrix}\alpha & \beta\\
\beta & -\alpha
\end{pmatrix}=\mathrm{i}
$$


***

$$
\begin{array}{ccccc}
 & \alpha^{2}+\beta^{2}=-1 & \begin{cases}
\alpha=\sqrt{-1}\\
\beta=0
\end{cases} & \begin{cases}
\alpha=\sqrt{-2}\\
\beta=1
\end{cases} & \beta=\alpha^{2},n\in\left\{ 1,2,4,5\right\} \\
1 & \begin{pmatrix}1 & 0\\
0 & 1
\end{pmatrix} & \begin{pmatrix}1 & 0\\
0 & 1
\end{pmatrix} & \begin{pmatrix}1 & 0\\
0 & 1
\end{pmatrix} & \begin{pmatrix}1 & 0\\
0 & 1
\end{pmatrix}\\
-1 & \begin{pmatrix}-1 & 0\\
0 & -1
\end{pmatrix} & \begin{pmatrix}-1 & 0\\
0 & -1
\end{pmatrix} & \begin{pmatrix}-1 & 0\\
0 & -1
\end{pmatrix} & \begin{pmatrix}-1 & 0\\
0 & -1
\end{pmatrix}\\
\mathrm{i} & \begin{pmatrix}\alpha & \beta\\
\beta & -\alpha
\end{pmatrix} & \begin{pmatrix}\sqrt{-1} & 0\\
0 & -\sqrt{-1}
\end{pmatrix} & \begin{pmatrix}\sqrt{-2} & 1\\
1 & -\sqrt{-2}
\end{pmatrix} & \begin{pmatrix}\mathrm{e}^{\pi\frac{n}{3}\sqrt{-1}} & \mathrm{e}^{\pi\frac{2n}{3}\sqrt{-1}}\\
\mathrm{e}^{\pi\frac{2n}{3}\sqrt{-1}} & -\mathrm{e}^{\pi\frac{n}{3}\sqrt{-1}}
\end{pmatrix}\\
-\mathrm{i} & \begin{pmatrix}-\alpha & -\beta\\
-\beta & \alpha
\end{pmatrix} & \begin{pmatrix}-\sqrt{-1} & 0\\
0 & \sqrt{-1}
\end{pmatrix} & \begin{pmatrix}-\sqrt{-2} & -1\\
-1 & \sqrt{-2}
\end{pmatrix} & \begin{pmatrix}-\mathrm{e}^{\pi\frac{n}{3}\sqrt{-1}} & -\mathrm{e}^{\pi\frac{2n}{3}\sqrt{-1}}\\
-\mathrm{e}^{\pi\frac{2n}{3}\sqrt{-1}} & \mathrm{e}^{\pi\frac{n}{3}\sqrt{-1}}
\end{pmatrix}\\
\mathrm{j} & \begin{pmatrix}0 & -1\\
1 & 0
\end{pmatrix} & \begin{pmatrix}0 & -1\\
1 & 0
\end{pmatrix} & \begin{pmatrix}0 & -1\\
1 & 0
\end{pmatrix} & \begin{pmatrix}0 & -1\\
1 & 0
\end{pmatrix}\\
-\mathrm{j} & \begin{pmatrix}0 & 1\\
-1 & 0
\end{pmatrix} & \begin{pmatrix}0 & 1\\
-1 & 0
\end{pmatrix} & \begin{pmatrix}0 & 1\\
-1 & 0
\end{pmatrix} & \begin{pmatrix}0 & 1\\
-1 & 0
\end{pmatrix}\\
\mathrm{k} & \begin{pmatrix}\beta & -\alpha\\
-\alpha & -\beta
\end{pmatrix} & \begin{pmatrix}0 & -\sqrt{-1}\\
-\sqrt{-1} & 0
\end{pmatrix} & \begin{pmatrix}1 & -\sqrt{-2}\\
-\sqrt{-2} & -1
\end{pmatrix} & \begin{pmatrix}\mathrm{e}^{\pi\frac{2n}{3}\sqrt{-1}} & -\mathrm{e}^{\pi\frac{n}{3}\sqrt{-1}}\\
-\mathrm{e}^{\pi\frac{n}{3}\sqrt{-1}} & -\mathrm{e}^{\pi\frac{2n}{3}\sqrt{-1}}
\end{pmatrix}\\
-\mathrm{k} & \begin{pmatrix}-\beta & \alpha\\
\alpha & \beta
\end{pmatrix} & \begin{pmatrix}0 & \sqrt{-1}\\
\sqrt{-1} & 0
\end{pmatrix} & \begin{pmatrix}-1 & \sqrt{-2}\\
\sqrt{-2} & 1
\end{pmatrix} & \begin{pmatrix}-\mathrm{e}^{\pi\frac{2n}{3}\sqrt{-1}} & \mathrm{e}^{\pi\frac{n}{3}\sqrt{-1}}\\
\mathrm{e}^{\pi\frac{n}{3}\sqrt{-1}} & \mathrm{e}^{\pi\frac{2n}{3}\sqrt{-1}}
\end{pmatrix}
\end{array}
$$

***

$$
\begin{aligned}
-1= & \alpha^{2}+\beta^{2}\\
\overset{\beta=\alpha^{2}}{=} & \alpha^{2}+\alpha^{4}\\
\alpha^{4}+\alpha^{2}+1= & 0,\alpha^{4}+\alpha^{2}+1=\left(\alpha^{2}+\alpha+1\right)\left(\alpha^{2}-\alpha+1\right)\\
\left(\alpha^{2}-1\right)\left(\alpha^{4}+\alpha^{2}+1\right)= & 0\\
\alpha^{6}-1= & 0\\
\alpha^{6}= & 1=\mathrm{e}^{2\pi k\sqrt{-1}},k\in\mathbb{Z}\\
\alpha= & \mathrm{e}^{2\pi\frac{n}{6}\sqrt{-1}},n\in\left\{ 0,1,2,3,4,5\right\} -\left\{ 0,3\right\} \\
= & \mathrm{e}^{\pi\frac{n}{3}\sqrt{-1}},n\in\left\{ 1,2,4,5\right\} 
\end{aligned}
$$

***

$$
\begin{array}{ccccc}
 & \alpha^{2}+\beta^{2}=-1 & \begin{cases}
\alpha=\sqrt{-1}\\
\beta=0
\end{cases} & \begin{cases}
\alpha=\sqrt{-2}\\
\beta=1
\end{cases} & \omega=\mathrm{e}^{i\pi\frac{n}{3}},n\in\left\{ 1,2,4,5\right\} \\
1 & \begin{pmatrix}1 & 0\\
0 & 1
\end{pmatrix} & \begin{pmatrix}1 & 0\\
0 & 1
\end{pmatrix} & \begin{pmatrix}1 & 0\\
0 & 1
\end{pmatrix} & \begin{pmatrix}1 & 0\\
0 & 1
\end{pmatrix}\\
-1 & \begin{pmatrix}-1 & 0\\
0 & -1
\end{pmatrix} & \begin{pmatrix}-1 & 0\\
0 & -1
\end{pmatrix} & \begin{pmatrix}-1 & 0\\
0 & -1
\end{pmatrix} & \begin{pmatrix}-1 & 0\\
0 & -1
\end{pmatrix}\\
\mathrm{i} & \begin{pmatrix}\alpha & \beta\\
\beta & -\alpha
\end{pmatrix} & \begin{pmatrix}i & 0\\
0 & -i
\end{pmatrix} & \begin{pmatrix}\sqrt{2}i & 1\\
1 & -\sqrt{2}i
\end{pmatrix} & \begin{pmatrix}\omega & \omega^{2}\\
\omega^{2} & -\omega
\end{pmatrix}\\
-\mathrm{i} & \begin{pmatrix}-\alpha & -\beta\\
-\beta & \alpha
\end{pmatrix} & \begin{pmatrix}-i & 0\\
0 & i
\end{pmatrix} & \begin{pmatrix}-\sqrt{2}i & -1\\
-1 & \sqrt{2}i
\end{pmatrix} & \begin{pmatrix}-\omega & -\omega^{2}\\
-\omega^{2} & \omega
\end{pmatrix}\\
\mathrm{j} & \begin{pmatrix}0 & -1\\
1 & 0
\end{pmatrix} & \begin{pmatrix}0 & -1\\
1 & 0
\end{pmatrix} & \begin{pmatrix}0 & -1\\
1 & 0
\end{pmatrix} & \begin{pmatrix}0 & -1\\
1 & 0
\end{pmatrix}\\
-\mathrm{j} & \begin{pmatrix}0 & 1\\
-1 & 0
\end{pmatrix} & \begin{pmatrix}0 & 1\\
-1 & 0
\end{pmatrix} & \begin{pmatrix}0 & 1\\
-1 & 0
\end{pmatrix} & \begin{pmatrix}0 & 1\\
-1 & 0
\end{pmatrix}\\
\mathrm{k} & \begin{pmatrix}\beta & -\alpha\\
-\alpha & -\beta
\end{pmatrix} & \begin{pmatrix}0 & -i\\
-i & 0
\end{pmatrix} & \begin{pmatrix}1 & -\sqrt{2}i\\
-\sqrt{2}i & -1
\end{pmatrix} & \begin{pmatrix}\omega^{2} & -\omega\\
-\omega & -\omega^{2}
\end{pmatrix}\\
-\mathrm{k} & \begin{pmatrix}-\beta & \alpha\\
\alpha & \beta
\end{pmatrix} & \begin{pmatrix}0 & i\\
i & 0
\end{pmatrix} & \begin{pmatrix}-1 & \sqrt{2}i\\
\sqrt{2}i & 1
\end{pmatrix} & \begin{pmatrix}-\omega^{2} & \omega\\
\omega & \omega^{2}
\end{pmatrix}
\end{array}
$$

$$
\mathbb{H}\rightarrow\mathcal{M}_{2\times2}\left(\mathbb{C}\right)
$$


### $\mathbb{H}\rightarrow\mathcal{M}_{4\times4}\left(\mathbb{R}\right)$

https://groupprops.subwiki.org/wiki/Linear_representation_theory_of_quaternion_group#Four-dimensional_irreducible_representation_over_a_non-splitting_field