# math {#nice-label}

- formula typesetting
    - TeX
        - LaTeX
            - pdfLaTeX
            - XeLaTeX
            - editor/tool:
                - LyX
                - OverLeaf
                - MathPix Snip
                - Micro$oft Office Word
    - MathML
    - MathJax: JavaScript
- symbolic computing
    - Maple:          by MapleSoft
    - Mathematica:    by Wolfram
- numeric computing
    - MatLab:         by MathWorks

[equivalence relation] \@ref(equivalence-relation)

[equivalence class] \@ref(equivalence-class)

[partition] \@ref(partition)


# equivalence relation {-}

<!-- \begin{CJK}{UTF8}{bsmi} -->
<!-- \begin{defn} -->














https://stackoverflow.com/questions/76240244/bookdown-conditional-display-of-text-and-code-blocks-latex-pdf-vs-html

::: {show-in="html"}

\begingroup
\fontfamily{ppl}\fontsize{1}{1}\selectfont
\begin{align*}
 & R\text{ is an equivalence relation over }A\times B\\
\Leftrightarrow & \begin{cases}
R=\sim=\left\{ \left\langle x,y\right\rangle \middle|x\sim y\right\} \subseteq A\times B & \left(\text{e}\right)\text{equivalence 等價}\\
\vdots & \vdots
\end{cases}\\
\Leftrightarrow & \begin{cases}
R=\left\{ \left\langle x,y\right\rangle \middle|xRy\right\} \subseteq A\times B & \left(R\right)\text{relation}\\
\forall\left\langle x,y\right\rangle \in R\left(xRx\right) & \left(r\right)\text{reflexive}\\
\forall\left\langle x,y\right\rangle \in R\left(xRy\Rightarrow yRx\right) & \left(s\right)\text{symmetric}\\
\forall\left\langle x,y\right\rangle ,\left\langle y,z\right\rangle \in R\left(\begin{cases}
xRy\\
yRz
\end{cases}\Rightarrow xRz\right) & \left(t\right)\text{transitive}
\end{cases}\Leftrightarrow\begin{cases}
R=\left\{ \left\langle x,y\right\rangle \middle|xRy\right\} \subseteq A\times B & \text{關係}\\
\forall\left\langle x,y\right\rangle \in R\left(\left\langle x,x\right\rangle \in R\right) & \text{自反}\\
\forall\left\langle x,y\right\rangle \in R\left(\left\langle y,x\right\rangle \in R\right) & \text{對稱}\\
\forall\left\langle x,y\right\rangle ,\left\langle y,z\right\rangle \in R\left(\left\langle x,z\right\rangle \in R\right) & \text{遞移}
\end{cases}
\end{align*}
\endgroup

:::

::: {show-in="pdf"}

\begin{CJK}{UTF8}{bsmi}等價關係 equivalence relation \label{def:equivalence-relation}
\end{CJK}
\begin{CJK}{UTF8}{bsmi}
\begin{align*}
 & R\text{ is an equivalence relation over }A\times B\\
\Leftrightarrow & \begin{cases}
R=\sim=\left\{ \left\langle x,y\right\rangle \middle|x\sim y\right\} \subseteq A\times B & \left(\text{e}\right)\text{equivalence 等價}\\
\vdots & \vdots
\end{cases}\\
\Leftrightarrow & \begin{cases}
R=\left\{ \left\langle x,y\right\rangle \middle|xRy\right\} \subseteq A\times B & \left(R\right)\text{relation}\\
\forall\left\langle x,y\right\rangle \in R\left(xRx\right) & \left(r\right)\text{reflexive}\\
\forall\left\langle x,y\right\rangle \in R\left(xRy\Rightarrow yRx\right) & \left(s\right)\text{symmetric}\\
\forall\left\langle x,y\right\rangle ,\left\langle y,z\right\rangle \in R\left(\begin{cases}
xRy\\
yRz
\end{cases}\Rightarrow xRz\right) & \left(t\right)\text{transitive}
\end{cases}\Leftrightarrow\begin{cases}
R=\left\{ \left\langle x,y\right\rangle \middle|xRy\right\} \subseteq A\times B & \text{關係}\\
\forall\left\langle x,y\right\rangle \in R\left(\left\langle x,x\right\rangle \in R\right) & \text{自反}\\
\forall\left\langle x,y\right\rangle \in R\left(\left\langle y,x\right\rangle \in R\right) & \text{對稱}\\
\forall\left\langle x,y\right\rangle ,\left\langle y,z\right\rangle \in R\left(\left\langle x,z\right\rangle \in R\right) & \text{遞移}
\end{cases}
\end{align*}
\end{CJK}
<!-- \end{defn} -->

:::


# equivalence class {-}

\begin{align*}
 & C\text{ is an equivalence class of }a\text{ on }A\\
\Leftrightarrow & \left[a\right]_{\sim}=C=\left\{ x\middle|\begin{cases}
a\in A\\
x\in A\\
x\sim a\\
\sim\text{ is an equivalence relation over }A\times A=A^{2}
\end{cases}\right\} \subseteq A\ne\emptyset\\
\Leftrightarrow & \left[a\right]=\left[a\right]_{\sim}=\left\{ x\middle|\begin{cases}
a\in A\\
x\in A\\
x\sim a\\
\sim\text{ is an equivalence relation on }A
\end{cases}\right\} \subseteq A\ne\emptyset\\
\Rightarrow & \left[a\right]_{\sim}=\left\{ x\middle|x\sim a\right\} \subseteq A\ne\emptyset
\end{align*}

where the definition of [equivalence relation] can be found in \@ref(equivalence-relation).

[number and reference equations]

\@ref(eq:eqclass)

\@ref(eq:emc)

\@ref(thm:pyth)


# partition {-}

\begin{align*}
 & \left\{ A_{i}\right\} _{i\in I}=\left\{ A_{i}\middle|i\in I\right\} \text{ is a partition of a set }A\\
\Leftrightarrow & \begin{cases}
\forall i\in I\left(A_{i}\ne\emptyset\right)\\
A=\bigcup\limits _{i\in I}A_{i}\\
\forall i,j\in I\left(i\ne j\Rightarrow A_{i}\cap A_{j}=\emptyset\right)
\end{cases}
\end{align*}

https://proofwiki.org/wiki/Definition:Set_Partition


# statistics


## covariance matrix 

@ccjou2014

### calculation

\begin{align*}
\mathrm{C}\left[\boldsymbol{X}\right]=\mathrm{Cov}\left[\boldsymbol{X}\right]=\mathrm{V}\left[\boldsymbol{X}\right]= & \mathrm{E}\left[\left[\boldsymbol{X}-\mathrm{E}\left(\boldsymbol{X}\right)\right]\left[\boldsymbol{X}-\mathrm{E}\left(\boldsymbol{X}\right)\right]^{\mathrm{T}}\right]\\
= & \mathrm{E}\left[\left[\boldsymbol{X}-\mathrm{E}\left(\boldsymbol{X}\right)\right]\left[\boldsymbol{X}^{\mathrm{T}}-\mathrm{E}\left(\boldsymbol{X}\right)^{\mathrm{T}}\right]\right]\\
= & \mathrm{E}\left[\boldsymbol{X}\boldsymbol{X}^{\mathrm{T}}-\mathrm{E}\left(\boldsymbol{X}\right)\boldsymbol{X}^{\mathrm{T}}-\boldsymbol{X}\mathrm{E}\left(\boldsymbol{X}\right)^{\mathrm{T}}+\mathrm{E}\left(\boldsymbol{X}\right)\mathrm{E}\left(\boldsymbol{X}\right)^{\mathrm{T}}\right]\\
= & \mathrm{E}\left[\boldsymbol{X}\boldsymbol{X}^{\mathrm{T}}\right]-\mathrm{E}\left[\mathrm{E}\left(\boldsymbol{X}\right)\boldsymbol{X}^{\mathrm{T}}\right]-\mathrm{E}\left[\boldsymbol{X}\mathrm{E}\left(\boldsymbol{X}\right)^{\mathrm{T}}\right]+\mathrm{E}\left[\mathrm{E}\left(\boldsymbol{X}\right)\mathrm{E}\left(\boldsymbol{X}\right)^{\mathrm{T}}\right]\\
= & \mathrm{E}\left[\boldsymbol{X}\boldsymbol{X}^{\mathrm{T}}\right]-\mathrm{E}\left(\boldsymbol{X}\right)\mathrm{E}\left[\boldsymbol{X}^{\mathrm{T}}\right]-\mathrm{E}\left[\boldsymbol{X}\right]\mathrm{E}\left(\boldsymbol{X}\right)^{\mathrm{T}}+\mathrm{E}\left(\boldsymbol{X}\right)\mathrm{E}\left(\boldsymbol{X}\right)^{\mathrm{T}}\\
= & \mathrm{E}\left[\boldsymbol{X}\boldsymbol{X}^{\mathrm{T}}\right]-\mathrm{E}\left(\boldsymbol{X}\right)\mathrm{E}\left(\boldsymbol{X}\right)^{\mathrm{T}}-\mathrm{E}\left(\boldsymbol{X}\right)\mathrm{E}\left(\boldsymbol{X}\right)^{\mathrm{T}}+\mathrm{E}\left(\boldsymbol{X}\right)\mathrm{E}\left(\boldsymbol{X}\right)^{\mathrm{T}}\\
= & \mathrm{E}\left[\boldsymbol{X}\boldsymbol{X}^{\mathrm{T}}\right]-\mathrm{E}\left(\boldsymbol{X}\right)\mathrm{E}\left(\boldsymbol{X}\right)^{\mathrm{T}}
\end{align*}

\begin{align*}
\boldsymbol{X}=\left[X\right]_{1\times1}=X\Rightarrow C\left(X\right)=\mathrm{C}\left[\boldsymbol{X}\right]= & \mathrm{E}\left[\boldsymbol{X}\boldsymbol{X}^{\mathrm{T}}\right]-\mathrm{E}\left(\boldsymbol{X}\right)\mathrm{E}\left(\boldsymbol{X}\right)^{\mathrm{T}}\\
= & \mathrm{E}\left[XX\right]-\mathrm{E}\left(X\right)\mathrm{E}\left(X\right)\\
= & \mathrm{E}\left(X^{2}\right)-\left[\mathrm{E}\left(X\right)\right]^{2}=\mathrm{V}\left(X\right)
\end{align*}

### $\mathrm{V}\left[\boldsymbol{X}+\boldsymbol{b}\right]=\mathrm{V}\left[\boldsymbol{X}\right]$

\begin{align*}
\mathrm{V}\left[\boldsymbol{X}+\boldsymbol{b}\right]= & \mathrm{E}\left[\left[\left(\boldsymbol{X}+\boldsymbol{b}\right)-\mathrm{E}\left(\boldsymbol{X}+\boldsymbol{b}\right)\right]\left[\left(\boldsymbol{X}+\boldsymbol{b}\right)-\mathrm{E}\left(\boldsymbol{X}+\boldsymbol{b}\right)\right]^{\mathrm{T}}\right]\\
\overset{\mathrm{E}\left(\boldsymbol{X}+\boldsymbol{b}\right)=\mathrm{E}\left(\boldsymbol{X}\right)+\boldsymbol{b}}{=} & \mathrm{E}\left[\left[\boldsymbol{X}+\boldsymbol{b}-\mathrm{E}\left(\boldsymbol{X}\right)-\boldsymbol{b}\right]\left[\boldsymbol{X}+\boldsymbol{b}-\mathrm{E}\left(\boldsymbol{X}\right)-\boldsymbol{b}\right]^{\mathrm{T}}\right]\\
= & \mathrm{E}\left[\left[\boldsymbol{X}-\mathrm{E}\left(\boldsymbol{X}\right)\right]\left[\boldsymbol{X}-\mathrm{E}\left(\boldsymbol{X}\right)\right]^{\mathrm{T}}\right]=\mathrm{V}\left[\boldsymbol{X}\right]
\end{align*}

### $\mathrm{V}\left[A\boldsymbol{X}\right]=A\mathrm{V}\left[\boldsymbol{X}\right]A^{\mathrm{T}}$

\begin{align*}
\mathrm{V}\left[A\boldsymbol{X}\right]= & \mathrm{E}\left[\left[\left(A\boldsymbol{X}\right)-\mathrm{E}\left(A\boldsymbol{X}\right)\right]\left[\left(A\boldsymbol{X}\right)-\mathrm{E}\left(A\boldsymbol{X}\right)\right]^{\mathrm{T}}\right]\\
\overset{\mathrm{E}\left(A\boldsymbol{X}\right)=A\mathrm{E}\left(\boldsymbol{X}\right)}{=} & \mathrm{E}\left[\left[A\boldsymbol{X}-A\mathrm{E}\left(\boldsymbol{X}\right)\right]\left[A\boldsymbol{X}-A\mathrm{E}\left(\boldsymbol{X}\right)\right]^{\mathrm{T}}\right]\\
= & \mathrm{E}\left[A\left[\boldsymbol{X}-\mathrm{E}\left(\boldsymbol{X}\right)\right]\left[A\left[\boldsymbol{X}-\mathrm{E}\left(\boldsymbol{X}\right)\right]\right]^{\mathrm{T}}\right]\\
= & \mathrm{E}\left[A\left[\boldsymbol{X}-\mathrm{E}\left(\boldsymbol{X}\right)\right]\left[\boldsymbol{X}-\mathrm{E}\left(\boldsymbol{X}\right)\right]^{\mathrm{T}}A^{\mathrm{T}}\right]\\
= & A\mathrm{E}\left[\left[\boldsymbol{X}-\mathrm{E}\left(\boldsymbol{X}\right)\right]\left[\boldsymbol{X}-\mathrm{E}\left(\boldsymbol{X}\right)\right]^{\mathrm{T}}\right]A^{\mathrm{T}}=A\mathrm{V}\left[\boldsymbol{X}\right]A^{\mathrm{T}}
\end{align*}

### $\mathrm{V}\left[A\boldsymbol{X}+\boldsymbol{b}\right]=A\mathrm{V}\left[\boldsymbol{X}\right]A^{\mathrm{T}}$

$$
\mathrm{V}\left[A\boldsymbol{X}+\boldsymbol{b}\right]=\mathrm{V}\left[A\boldsymbol{X}\right]=A\mathrm{V}\left[\boldsymbol{X}\right]A^{\mathrm{T}}
$$
